## 3. Induction

#### 3.1
`P(1)` yields an even number: $2 = 1(1+1)$  
`P(n)` always gives an even number since multiplying an even number and an odd number yields an even number:  
$1(1+1),2(2+1),3(3+1)\dots = 2, 6, 12 \dots$


#### 3.2
`P(1)` yields the same number: $1=1 = \frac{1(1+1)}{2}$  
Then `P(n)` $1+2+3+\dots +n = \frac{n(n+1)}{2}$  
$1+2+3+\dots +n+n(n+1) = \frac{n(n+1)}{2} + (n+1) = \frac{n(n+1)}{2} + \frac{2(n+1)}{2} = \frac{(n+1)(n+2)}{2}$  


#### 3.3
The youngest one of all  


#### 3.4
![square](https://github.com/jonathantorres/bookshelf/blob/master/math/img/3.4.jpg)


#### 3.5
`P(3)` yields the same number: $1\cdot 2 + 2\cdot 3 = \frac{(3-1)\cdot 3\cdot(3+1)}{3}$  
Then `P(n)` $1\cdot 2 + 2\cdot 3+\dots +(n-1)\cdot n = \frac{(n-1)\cdot n \cdot (n+1)}{3}$  
$1\cdot 2 + 2\cdot 3 +\dots + (n-1) \cdot n + n\cdot (n+1) = \frac{n\cdot (n+1) \cdot (n+2)}{3}$  


#### 3.6
`P(4)` with an even number: $1+n=2+n-1\dots = (\frac{n}{2}-1)+\frac{n}{2}=n+1 = \frac{n}{2}(n+1) = \frac{n(n+1)}{2}$  


#### 3.7
`P(4)` with an even number: $1+(2n-1)=3+(2n-3)=\dots =(n-1)+(n+1)=2n=\frac{n}{2}(2n)=n^2$  


#### 3.8
`P(3)` yields the same number: $1+4+9=\frac{3(3+1)(2\cdot 3+1)}{6}$  
Then `P(n)` $1+4+9+\dots +n^2 = \frac{n(n+1)(2n+1)}{6}=1+2^2+3^2+\dots (n-1)^2=\frac{(n-1)(n)(2n-1)}{6}$  


#### 3.9
`P(3)` yields the same number: $1+2+4=2^3-1$  
Then `P(n)` $2^0+2^1+2^2+\dots +2^{(n-1)}=2^n-1=2^0+2^1+2^2+\dots +2^{(n-2)}=2^{(n-1)}-1$  


#### 3.10
`P(3)` is a string `S` of length `n` with `k` letters = $K^n$  
Then `P(n,k)` $K^{n-1}\cdot K = K^n$  
`P(3)` is the permutations of a set `S` with `n` elements = $n!$  
Then `P(n)` $(n-1)!\cdot n=n!$


#### 3.11
`P(3)` is when `n` people shake hands with each other = $\frac{n(n-1)}{2}$ handshakes  
Then `P(n)` $\frac{(n-1)(n-2)}{2}+n-1=\frac{n(n-1)}{2}$


#### 3.12
`n-1` is not always odd, if we multiply an odd number and an even one we get an even number. If `(n-1)` gets an even number then multiplying two even numbers yields an even number.


#### 3.13
There are at least 4 lines in the proof, but only $n=1,2$ are checked


#### 3.14
`P(3)` is a set of `n` lines that divides the plane in $\frac{1+n(n+1)}{2}$ regions  
Then `P(n)` $\frac{1+(n-1)(n)}{2}=\frac{1+(n^2)-n}{2}$
