## 6. Fibonacci Numbers

#### 6.1
We need the two previous values to compute the next


#### 6.2
$F_{n+1} = F_n + F_{n-1}$


#### 6.3
`P(1)` $F_{3(1)} = F_3 = 2$ is even  
`P(n)` $F_{3n}$ Two odd members are followed by an even member  


#### 6.4
Four members non-divisible by 5 are followed by a member divisible by 5  


#### 6.5
a) If $n\geq 3$ then $F_1 + F_3 + F_5 + \dots + F_{2n-1} = F_{2n} = (F_1 + F_3 + \dots + F_{2n-3}) + F_{2n-1} = F_{2n-2} + F_{2n-1}$  
b) If $n\geq 3$ then $F_0 - F_1 + F_2 - F_3 + \dots - F_{2n-1} + F_{2n} = F_{2n-1} - 1 = F_0 - F_1 + F_2 - F_3 + \dots - F_{2n-1} + F{2n}(F_0-F_1+F_2-\dots +F_{2n-2}) - (F_{2n-1 + F_{2n}}) = (F_{2n-3} -1) + F_{2n-2}$  
c) If $n\geq 3$ then $F^2_0 + F^2_1 + F^2_2 + \dots + F^2_n(F^2_0+F^2_1+\dots +F^2_{n-1}) + F^2_n = F_{n-1} F_n + F^2_n = F_n(F_{n-1} + F_n)$  
d) If $n\geq 3$ then $F_{n-1} F_{n+1} - F^2_n = F_{n-1} (F_{n-1} + F_n) - F^2_n = F^2_{n-1} + F_n(F_{n-1} - F_n) = F^2_{n-1} - F_n F_{n-2}$  


#### 6.6
a) A Fibonacci sequence
b) $\binom{n}{0} + \binom{n-1}{1} + \binom{n-2}{2} + \dots + \binom{n-k}{k} = F_{n-1}$


#### 6.7
No, I don't think so. A diagonal creates an extra square


#### 6.8
$F_n = F_{n-1} + F_{n+2}$


#### 6.9
$H_n = (\frac{1+\sqrt{5}}{2})^{n+1} + \frac{1-\sqrt{5}}{2}^{n+1}$


#### 6.10
$I_n = \frac{1}{2\sqrt{5}} ((2+\sqrt{5})^n - (2-\sqrt{5})^n)$

